add declassify

coq/two/Lambda.v
@@ -33,7 +33,8 @@ Inductive term : Type :=
   | TNat : nat -> term
   | TVar : nat -> term
   | TAbs : term -> term
-  | TApp : term -> term -> term.
+  | TApp : term -> term -> term
+  | TDecl : term -> term -> term.
 
 Inductive atom : Type :=
   | Atom : value -> two -> atom
@@ -53,6 +54,73 @@ Fixpoint lookup (e : env) (n : nat) : option atom :=
         | S n' => lookup e' n'
       end
   end.
+
+Section Indistinguishability.
+
+  Require Import Program.Tactics.
+  Require Import MyList.
+  
+  Context (L : two)
+          (P : value -> value -> Prop)
+          (Prefl : forall x, P x x).
+  
+  Fixpoint atom_LPequiv a1 a2 : Prop :=
+    match a1, a2 with
+      | Atom v1 l1, Atom v2 l2 =>
+        (L = Bottom2 /\ l1 = l2 /\ l1 = Top2 /\
+         match v1, v2 with
+           | VNat n1, VNat n2 => P v1 v2
+           | VClos e1 t1, VClos e2 t2 => value_LPequiv v1 v2
+           | _, _ => True
+         end) \/
+        (L = Bottom2 /\ l1 = l2 /\ l1 = Bottom2 /\ value_LPequiv v1 v2) \/
+        (L = Top2 /\ l1 = l2 /\ value_LPequiv v1 v2)
+    end
+  with value_LPequiv v1 v2 : Prop :=
+         match v1, v2 with
+           | VBool b1, VBool b2 => b1 = b2
+           | VNat n1, VNat n2 => n1 = n2
+           | VClos e1 t1, VClos e2 t2 =>
+             list_forall2 atom_LPequiv e1 e2 /\ t1 = t2
+           | VBool _, _ | VNat _, _ | VClos _ _, _ => False
+         end.
+
+  Definition env_LPequiv : env -> env -> Prop :=
+    list_forall2 atom_LPequiv.
+
+  Lemma atom_LPequiv_lab_inv :
+    forall v1 v2 l1 l2,
+      atom_LPequiv (Atom v1 l1) (Atom v2 l2) ->
+      l1 = l2.
+  Proof.
+    intros. inversion H; inversion H0; destruct_conjs; auto.
+  Qed.
+
+  Lemma atom_LPequiv_raise :
+    forall v1 v2,
+      atom_LPequiv (Atom v1 Bottom2) (Atom v2 Bottom2) ->
+      atom_LPequiv (Atom v1 Top2) (Atom v2 Top2).
+  Proof.
+    intros v1 v2 H. destruct L.
+    - destruct v1; destruct v2; destruct H; destruct H; destruct_conjs;
+      inversion H; try inversion H1; subst; auto.
+      + destruct H2. left. auto.
+      + right. right. auto.
+      + destruct H2. left. auto.
+      + right. right. auto.
+      + left. auto.
+      + right. right. auto.
+    - destruct v1; destruct v2; destruct H; destruct H; destruct_conjs;
+      inversion H; inversion H1; inversion H2; subst.
+      + destruct H2. left. auto.
+      + right. right. auto.
+      + left. auto.
+      + right. right. auto.
+      + left. auto.
+      + right. right.  auto.
+  Qed.
+
+End Indistinguishability.
 
 Definition eval_kl : nat * nat -> two -> (value -> value -> Prop) ->
                      two -> env -> term -> atom -> Prop.
@@ -79,8 +147,22 @@ Definition eval_kl : nat * nat -> two -> (value -> value -> Prop) ->
                          eval L P pc e t1 (Atom (VClos e1' t1') l1) /\
                          eval L P pc e t2 a2 /\
                          eval L P l1 (a2 :: e1') t1' a
-              end)).
-  unfold pair_lt. simpl. omega.
+                | TDecl t1 t2 =>
+                  if Compare_dec.zerop (fst kl) then False
+                  else let eval := eval_kl (fst kl - 1, snd kl) _ in
+                       exists e1' t1' l1 a2 v3 l3,
+                         eval L P pc e t1 (Atom (VClos e1' t1') l1) /\
+                         eval L P pc e t2 a2 /\
+                         eval L P l1 (a2 :: e1') t1' (Atom v3 l3) /\
+                         if bottomp l3 then a = Atom v3 Bottom2
+                         else let eval := eval_kl (snd kl, fst kl - 1) _ in
+                              (forall a2' e2' v3',
+                                 env_LPequiv L P (a2 :: e1') (a2' :: e2') ->
+                                 eval L P l1 (a2' :: e2') t1' (Atom v3' Top2) ->
+                                 value_LPequiv L P v3 v3') /\
+                              a = Atom v3 Bottom2
+              end));
+  unfold pair_lt; simpl; omega.
 Defined.
 
 Lemma eval_kl_eq :
@@ -105,6 +187,20 @@ Lemma eval_kl_eq :
                  eval L P pc e t1 (Atom (VClos e1' t1') l1) /\
                  eval L P pc e t2 a2 /\
                  eval L P l1 (a2 :: e1') t1' a
+        | TDecl t1 t2 =>
+          if Compare_dec.zerop (fst kl) then False
+          else let eval := eval_kl (fst kl - 1, snd kl) in
+               exists e1' t1' l1 a2 v3 l3,
+                 eval L P pc e t1 (Atom (VClos e1' t1') l1) /\
+                 eval L P pc e t2 a2 /\
+                 eval L P l1 (a2 :: e1') t1' (Atom v3 l3) /\
+                 if bottomp l3 then a = Atom v3 Bottom2
+                 else let eval := eval_kl (snd kl, fst kl - 1) in
+                      (forall a2' e2' v3',
+                         env_LPequiv L P (a2 :: e1') (a2' :: e2') ->
+                         eval L P l1 (a2' :: e2') t1' (Atom v3' Top2) ->
+                         value_LPequiv L P v3 v3') /\
+                      a = Atom v3 Bottom2
       end.
 Proof.
   intro kl.
@@ -117,16 +213,23 @@ Proof.
   apply functional_extensionality; intro e.
   apply functional_extensionality; intro t.
   apply functional_extensionality; intro a.
-  destruct t; try reflexivity.
-  destruct x1; auto; simpl.
-  apply functional_extensionality_ex; intro e1'.
-  apply functional_extensionality_ex; intro t1'.
-  apply functional_extensionality_ex; intro l1.
-  apply functional_extensionality_ex; intro a2.
+  destruct t; try reflexivity;
   assert (H': forall (y : nat * nat), f y = g y) by
-      (intro; apply functional_extensionality; apply H);
-    rewrite H'.
-  reflexivity.
+      (intro; apply functional_extensionality; apply H).
+  - destruct x1; auto; simpl.
+    apply functional_extensionality_ex; intro e1'.
+    apply functional_extensionality_ex; intro t1'.
+    apply functional_extensionality_ex; intro l1.
+    apply functional_extensionality_ex; intro a2.
+    rewrite H'. reflexivity.
+  - destruct x1; auto; simpl.
+    apply functional_extensionality_ex; intro e1'.
+    apply functional_extensionality_ex; intro t1'.
+    apply functional_extensionality_ex; intro l1.
+    apply functional_extensionality_ex; intro a2.
+    apply functional_extensionality_ex; intro v3.
+    apply functional_extensionality_ex; intro l3.
+    destruct l3; rewrite H'; simpl; try rewrite H'; reflexivity.
 Qed.
 
 Lemma eval_k_bool :
@@ -203,4 +306,67 @@ Proof.
     replace (k - 0) with k in * by omega.
     exists k. exists e1'. exists t1'. exists l1. exists a2.
     split; try split; try split; assumption.
+Qed.
+
+Lemma eval_kl_decl1 :
+  forall k l L P pc e t1 t2 e1' t1' l1 a2 v3,
+    eval_kl (k, l) L P pc e t1 (Atom (VClos e1' t1') l1) ->
+    eval_kl (k, l) L P pc e t2 a2 ->
+    eval_kl (k, l) L P l1 (a2 :: e1') t1' (Atom v3 Bottom2) ->
+    eval_kl (S k, l) L P pc e (TDecl t1 t2) (Atom v3 Bottom2).
+Proof.
+  intros. rewrite eval_kl_eq. simpl.
+  replace (k - 0) with k by omega.
+  exists e1'. exists t1'. exists l1. exists a2. exists v3. exists Bottom2.
+  split; try split; try split; simpl; auto.
+Qed.
+
+Lemma eval_kl_decl2 :
+  forall k l L P pc e t1 t2 e1' t1' l1 a2 v3,
+    eval_kl (k, l) L P pc e t1 (Atom (VClos e1' t1') l1) ->
+    eval_kl (k, l) L P pc e t2 a2 ->
+    eval_kl (k, l) L P l1 (a2 :: e1') t1' (Atom v3 Top2) ->
+    (forall a2' e2' v3',
+       env_LPequiv L P (a2 :: e1') (a2' :: e2') ->
+       eval_kl (l, k) L P l1 (a2' :: e2') t1' (Atom v3' Top2) ->
+       value_LPequiv L P v3 v3') ->
+    eval_kl (S k, l) L P pc e (TDecl t1 t2) (Atom v3 Bottom2).
+Proof.
+  intros. rewrite eval_kl_eq. simpl.
+  replace (k - 0) with k by omega.
+  exists e1'. exists t1'. exists l1. exists a2. exists v3. exists Top2.
+  split; try split; try split; simpl; auto.
+Qed.
+
+Lemma eval_kl_decl_inv :
+  forall k l L P pc e t1 t2 a,
+    eval_kl (k, l) L P pc e (TDecl t1 t2) a ->
+    (exists k' e1' t1' l1 a2 v3,
+       k = S k' /\
+       eval_kl (k', l) L P pc e t1 (Atom (VClos e1' t1') l1) /\
+       eval_kl (k', l) L P pc e t2 a2 /\
+       eval_kl (k', l) L P l1 (a2 :: e1') t1' (Atom v3 Bottom2) /\
+       a = Atom v3 Bottom2) \/
+    (exists k' e1' t1' l1 a2 v3,
+       k = S k' /\
+       eval_kl (k', l) L P pc e t1 (Atom (VClos e1' t1') l1) /\
+       eval_kl (k', l) L P pc e t2 a2 /\
+       eval_kl (k', l) L P l1 (a2 :: e1') t1' (Atom v3 Top2) /\
+       (forall a2' e2' v3',
+          env_LPequiv L P (a2 :: e1') (a2' :: e2') ->
+          eval_kl (l, k') L P l1 (a2' :: e2') t1' (Atom v3' Top2) ->
+          value_LPequiv L P v3 v3') /\
+       a = Atom v3 Bottom2).
+Proof.
+  intros.
+  rewrite eval_kl_eq in H.
+  destruct k; simpl in H.
+  - inversion H.
+  - destruct H as [e1' [t1' [l1 [a2 [v3 [l3 [H1 [H2 [H3 H4]]]]]]]]].
+    replace (k - 0) with k in * by omega.
+    destruct l3; simpl in H4.
+    + left.
+      exists k. exists e1'. exists t1'. exists l1. exists a2. exists v3. auto.
+    + right.
+      exists k. exists e1'. exists t1'. exists l1. exists a2. exists v3. auto.
 Qed.
